Started the proof for well formed traces

Safety.v
@@ -1,4 +1,5 @@
 From Coq Require Import Init.Nat.
+From Coq Require Import Lists.List.
 
 From Elo Require Export Array.
 From Elo Require Export Map.
@@ -6,91 +7,93 @@ From Elo Require Export Map.
 From Elo Require Export Core.
 From Elo Require Export Properties.
 
-Reserved Notation "m / ths '==[' f ']==>+' m' / ths'"
-  (at level 40, ths at next level, f at next level, m' at next level).
+Inductive trace : list ceffect -> mem -> list tm -> Prop :=
+  | trace_nil : forall main T,
+    nil / empty |-- main is T ->
+    trace (CEF_None 0 :: nil) nil (main :: nil)
 
-Inductive multistep (f : ceffect -> Prop) :
-  mem -> list tm -> mem -> list tm -> Prop :=
-
-  | multistep_first : forall m m' ths ths' ceff,
-    f ceff ->
+  | trace_cons : forall m m' ths ths' ceff ceffs,
+    trace ceffs  m  ths ->
     m / ths ==> m' / ths' # ceff ->
-    m / ths ==[f]==>+ m' / ths'
-
-  | multistep_step : forall m1 m m2 ths1 ths ths2 ceff,
-    f ceff ->
-    m1 / ths1 ==> m / ths # ceff ->
-    m  / ths  ==[f]==>+ m2 / ths2 ->
-    m1 / ths1 ==[f]==>+ m2 / ths2
-
-  where "m / ths '==[' f ']==>+' m' / ths'" := (multistep f m ths m' ths').
-
-Reserved Notation "m / ths '==[' f ']==>+' m' / ths'"
-  (at level 40, ths at next level, f at next level, m' at next level).
-
-Inductive sequence : list ceffect -> mem -> list tm -> Prop :=
-  | sequence_nil : forall main,
-    sequence (CEF_None 0 :: nil) nil (main :: nil)
-
-  | sequence_cons : forall m m' ths ths' ceff ceffs,
-    m / ths ==> m' / ths' # ceff ->
-    sequence ceffs  m  ths ->
-    sequence (ceff :: ceffs) m' ths'
+    trace (ceff :: ceffs) m' ths'
   .
 
-Definition is_same_thread ceff i :=
-  match ceff with
-  | CEF_None  j
-  | CEF_Alloc j _
-  | CEF_Load  j _
-  | CEF_Store j _
-  | CEF_Spawn j   => i =? j
+(* TODO : tem que ser uma relação indutiva! *)
+Fixpoint no_concurrent_write ceffs i addr :=
+  match ceffs with
+  | nil => True
+
+  | CEF_Store i' addr' :: ceffs =>
+    (addr <> addr' \/ i = i') /\ (no_concurrent_write ceffs i addr)
+
+  | _ :: ceffs => no_concurrent_write ceffs i addr
   end.
 
-Definition is_write ceff addr :=
-  match ceff with
-  | CEF_Store _ addr' => addr =? addr'
-  | _ => false
-  end.
+Inductive well_formed_trace : list ceffect -> Prop :=
+  | well_formed_trace_nil :
+    well_formed_trace nil
 
-Definition is_not_concurrent_write (i addr : nat) (ceff : ceffect) :=
-  False.
+  | well_formed_trace_none : forall i ceffs,
+    well_formed_trace ceffs ->
+    well_formed_trace (CEF_None i :: ceffs)
 
-Theorem aux : forall m1 m2 m3 ths1 ths2 ths3 i addr,
-  m1 / ths1 ==> m2 / ths2 # (CEF_Load i addr) ->
-  m2 / ths2 ==[is_not_concurrent_write i addr]==>+ m3 / ths3.
+  | well_formed_trace_alloc : forall i addr ceffs,
+    well_formed_trace ceffs ->
+    well_formed_trace (CEF_Alloc i addr :: ceffs)
+
+  | well_formed_trace_load : forall i addr ceffs,
+    well_formed_trace ceffs ->
+    well_formed_trace (CEF_Load i addr :: ceffs)
+
+  | well_formed_trace_store : forall i addr ceffs,
+    well_formed_trace ceffs ->
+    no_concurrent_write ceffs i addr ->
+    well_formed_trace (CEF_Store i addr :: ceffs)
+
+  | well_formed_trace_spawn : forall i ceffs,
+    well_formed_trace ceffs ->
+    well_formed_trace (CEF_Spawn i :: ceffs)
+  .
+
+Lemma traces_are_well_typed : forall m ths ceffs,
+  trace ceffs m ths ->
+  exists mt, well_typed_program mt m ths.
 Proof.
-Admitted.
+  intros * Htrace. induction Htrace as [| ? ? ? ? ? ? ? [mt Hprog]].
+  - exists nil. split.
+    + split; trivial. destruct i; eauto using @typeof.
+    + intros i. unfold get_tm. simpl; destruct i;
+      try destruct i; eauto using @typeof. 
+  - assert (exists mt',
+      mt' extends mt /\
+      well_typed_program mt' m' ths') as [? [_ ?]];
+    eauto using preservation.
+Qed.
+
+Theorem traces_are_well_formed : forall ceffs m ths,
+  trace ceffs m ths ->
+  well_formed_trace ceffs.
+Proof.
+  intros ?. induction ceffs as [| ceff ceffs IH]; intros * Htrace.
+  - inversion Htrace.
+  - inversion Htrace; subst;
+    try destruct ceff; eauto using well_formed_trace.
+    eapply well_formed_trace_store; eauto.
+Qed.
 
 
 
-Inductive before : list tm -> list tm -> Prop :=
-  | todo : forall i j eff eff' m m' ths ths',
-    i < j ->
-    sequence i eff  m  ths  ->
-    sequence j eff' m' ths' ->
-    before ths ths'
-  .
 
-Definition synchronize (threads : list tm) (i j : nat) : Prop := False.
 
-Definition happens_before (threads : list tm) i j : Prop :=
-  if i =? j then i < j else synchronize threads i j.
 
-Definition data_race := forall (threads : list tm) i j,
-  (is_write (get_tm threads i) \/ is_write (get_tm threads j)) /\
-  ~ happens_before threads i j.
 
-(*
-Inductive happens_before' : mem -> tm -> mem -> tm -> Prop :=
-  | HB_Step : forall m m' t t',
-    m / t -->* m' / t' ->
-    happens_before' m t m' t'
-  .
-*)
 
-(*
-  Invariant:
-    At any time during program execution, each thread or monitor can only
-    access memory locations that are either local or safe.
-*)
+
+
+
+
+
+
+
+
+
